again but with inductive propositions

StackLean/Basic.lean
@@ -59,198 +59,109 @@ inductive Slot where
 instance : LawfulBEq Var := inferInstance
 instance : LawfulBEq Slot := inferInstance
 
--- Stacks ---
-
-abbrev Stack (sz : Nat):= { l : List Slot // l.length = sz}
-
-
-def Stack.vars (s : Stack sz) : LSet Var :=
-  let unwrap := λ s =>
-    match s with
-      | .Var v => some v
-      | _ => none
-
-  s.val |> List.filterMap unwrap |> LSet.ofList
-
 --- Targets ---
 
 -- A target is a specification of a desired shuffle outcome
-structure Target (nargs : Nat) where
+structure Target where
   -- a concrete args section that must have a specific order and multiplicity
-  args : Stack nargs
+  args : List Slot
   -- an abstract tail section that is a set of variables that must remain live for downstream ops
   liveOut : LSet Var
 
-def Target.surplus (target : Target nargs) (stack : Stack sz) (slot : Slot) : Prop :=
-  let target_args_count := target.args.val.count slot
-  let stack_head_count := stack.val |> List.take target.args.val.length |> List.count slot
-  match slot with
-  | .Var v => target_args_count < stack_head_count ∧ v ∈ target.liveOut
-  | .Lit _ => target_args_count < stack_head_count
-  | .Junk => True
+--- Stacks ---
 
-instance (target : Target nargs) (stack : Stack sz) (slot : Slot) : Decidable (target.surplus stack slot) := by
-  unfold Target.surplus
-  match slot with
-  | .Var v => exact inferInstance
-  | .Lit _ => exact inferInstance
-  | .Junk => exact isTrue trivial
+inductive Stack where
+  | Lit : (stk : List Slot) → Stack
+  | Swap : Nat → Stack → Stack
+  | Dup : Nat → Stack → Stack
+  | Pop : Stack → Stack
+  | Push : Word → Stack → Stack
+  | MarkJunk : Nat → Stack → Stack
 
---- Stack Manipulation ---
-
--- The operations that can be applied to a stack of a given size
-inductive Op : Nat → Type where
-  -- swap0 is a noop, the others match the evm
-  | Swap : (_ : szin > 0) → Fin (min 17 szin) → Op szin
-  -- dupn => evm dup(n + 1)
-  | Dup : (_ : szin > 0) → Fin (min 16 szin) → Op szin
-  | Pop : (_ : szin > 0) → Op szin
-  | Push : Word → Op szin
-  | MarkJunk : Fin szin → Op szin
-
--- The effect an operation has on the size of a stack
-@[reducible, simp]
-def sizeAfter (szin : Nat) (op : Op szin) : Nat := match op with
-  | .Swap _ _ => szin
-  | .Dup _ _ => szin + 1
-  | .Pop _ => szin - 1
-  | .Push _ => szin + 1
-  | .MarkJunk _ => szin
-
-def Stack.apply (stack : Stack szin) (op : Op szin) : Stack (sizeAfter szin op) :=
-  have : stack.val.length = szin := stack.property
-  match op with
-    | .Swap _ idx =>
-        have : idx < stack.val.length := by omega
-
-        let s := stack.val.set 0 stack.val[idx]
-        have : s.length = stack.val.length := by simp_all only [Fin.getElem_fin, List.length_set, s]
-
-        ⟨s.set (idx) stack.val[0], by simp_all⟩
-    | .Dup _ idx => ⟨stack.val[idx] :: stack.val, by simp_all⟩
-    | .Pop _ => ⟨stack.val.tail, by simp_all⟩
-    | .Push val => ⟨.Lit val :: stack.val, by simp_all⟩
-    | .MarkJunk idx =>
-      have : idx < stack.val.length := by omega
-      ⟨stack.val.set idx .Junk, by simp_all⟩
-
-inductive Stack' where
-  | Lit : (stk : List Slot) → Stack'
-  | Swap : Stack' → Nat → Stack'
-  | Dup : Stack' → Nat → Stack'
-  | Pop : Stack' → Stack'
-  | Push : Stack' → Word → Stack'
-  | MarkJunk : Stack' → Nat → Stack'
-
-inductive Stack'.eval : Stack' → (List Slot) → Prop where
-  | Lit : Stack'.eval (.Lit s) s
+inductive Stack.eval : Stack → (List Slot) → Prop where
+  | Lit : Stack.eval (.Lit s) s
   | Swap
-    : Stack'.eval s res
+    : Stack.eval s res
     → (hlen : res.length > idx)
     → (hlo : 0 < idx)
     → (hhi : idx < 17)
-    → Stack'.eval (.Swap s idx) ((res.set 0 res[idx]).set idx res[0])
+    → Stack.eval (.Swap idx s) ((res.set 0 res[idx]).set idx res[0])
   | Dup
-    : Stack'.eval s res
+    : Stack.eval s res
     → (hlen : idx < res.length)
     → (hlo : 1 ≤ idx)
     → (hhi : idx < 17)
-    → Stack'.eval (.Dup s idx) (res[idx] :: res)
+    → Stack.eval (.Dup idx s) (res[idx] :: res)
   | Pop
-    : Stack'.eval s res
+    : Stack.eval s res
     → (hlen : 0 < res.length)
-    → Stack'.eval (.Pop s) res.tail
+    → Stack.eval (.Pop s) res.tail
   | Push
-    : Stack'.eval s res
-    → Stack'.eval (.Push s word) (.Lit word :: res)
+    : Stack.eval s res
+    → Stack.eval (.Push word s) (.Lit word :: res)
   | MarkJunk
-    : Stack'.eval s res
+    : Stack.eval s res
     → (hlen : idx < res.length)
-    → Stack'.eval (.MarkJunk s idx) (res.set idx .Junk)
+    → Stack.eval (.MarkJunk idx s) (res.set idx .Junk)
 
 
 -- apply theorems --
 
+-- dup grows stack size by 1
+theorem apply_dup_grows_stack (stack : List Slot) (idx : Nat) (heval : Stack.eval (.Dup idx (.Lit stack)) res) : res.length = stack.length + 1 := match heval with
+  | .Dup .Lit hlen hlo hhi => by simp_all
+
+
 -- applying swap at the same idx twice is a noop
-theorem apply_swap_inv (sz : Nat) (hsz : sz > 0) (stack : Stack sz) (idx : Fin (min 17 sz)):
-  (stack.apply (.Swap hsz idx)).apply (.Swap hsz idx) = stack := by
-    simp_all [Stack.apply, List.getElem_set]
+theorem apply_swap_inv (stack : List Slot) (idx : Nat) (heval : Stack.eval (.Lit stack |> .Swap idx |> .Swap idx) res) : res = stack := match heval with
+  | .Swap (.Swap .Lit hlen' hlo' hhi') hlen hlo hhi => by
+    simp_all [List.getElem_set]
     split_ifs
     · simp_all
     · ext i
       simp_all [List.getElem?_set]
       split_ifs <;> simp_all
-
--- swap does not change the length of the stack
-theorem apply_swap_length (sz : Nat) (hsz : sz > 0) (stack : Stack sz) (idx : Fin (min 17 sz)) :
-  (stack.apply (.Swap hsz idx)).val.length = sz := by
-    simp [Stack.apply, stack.property]
-
--- swap switches the elem at idx with the elem at 0
-theorem apply_swap_positions_switched (sz: Nat) (hsz : sz > 0) (stack : Stack sz) (idx : Fin (min 17 sz)) :
-  ∃ (s' : Stack sz), stack.apply (.Swap hsz idx) = s' ∧ s'.val[0] = stack.val[idx] ∧ s'.val[idx]? = some stack.val[0] := by
-  have : idx < stack.val.length := by omega
-  simp_all [Stack.apply, List.getElem_set]
-
--- dup grows stack size by 1
-theorem apply_dup_grows_stack (sz : Nat) (hsz: sz > 0) (stack : Stack sz) (idx : Fin (min 16 sz)) :
-  (stack.apply (.Dup hsz idx)).val.length = (stack.val.length + 1) := by simp [Stack.apply]
-
--- the stack head is the same as the element at idx after applying (dup idx)
-theorem apply_dup_stack_top_eq_idx (sz : Nat) (hsz: sz > 0) (stack : Stack sz) (idx : Fin (min 16 sz)) :
-  (stack.apply (.Dup hsz idx)).val[0]'(by simp [Stack.apply]) = (stack.val[idx]) := by simp [Stack.apply]
-
--- the tail of the new stack is the same as the starting stack after applying (dup idx)
-theorem apply_dup_stack_tail_eq_prev (sz : Nat) (hsz : sz > 0) (stack : Stack sz) (idx : Fin (min 16 sz)) :
-  (stack.apply (.Dup hsz idx)).val.tail = stack := by simp [Stack.apply]
-
--- the result of applying pop is the same as the tail of the input stack
-theorem apply_pop_eq_prev_stack_tail (sz : Nat) (hsz : sz > 0) (stack : Stack sz) :
-  stack.apply (.Pop hsz) = stack.val.tail := by simp [Stack.apply]
-
--- TODO: push / markjunk theorems
+      exact List.getElem_eq_iff ?_
 
 --- Stack Shuffling ---
 
 inductive ShuffleResult where
   | StackTooDeep
   | ForbiddenState
-  | ResultStack (sz : Nat) (ops : List (Σ s, Op s)) (stack: Stack sz)
+  | ResultStack (start : List Slot) (finish : List Slot) (valid : Stack.eval (.Lit start) finish)
 
 @[simp]
-abbrev stack_is_large_enough (sz : Nat) (nargs : Nat) (target : Target nargs) : Prop := sz ≥ nargs + target.liveOut.val.length
+abbrev stack_is_large_enough (stack : List Slot) (target : Target) : Prop := stack.length ≥ target.args.length + target.liveOut.val.length
 
 @[simp]
-abbrev args_is_correct (sz : Nat) (stack: Stack sz) (nargs : Nat) (target : Target nargs) : Prop :=
-  have : target.args.val.length = nargs := target.args.property
-  have : stack.val.length = sz := stack.property
-  have hidx : (hle : stack_is_large_enough sz nargs target) -> ∀ i, i < nargs → i < stack.val.length := by omega
-  have thidx : ∀ i, i < nargs → i < target.args.val.length := by omega
+abbrev args_is_correct (stack: List Slot) (target : Target) : Prop :=
+  have hidx : (hle : stack_is_large_enough stack target) -> ∀ i, i < target.args.length → i < stack.length := by omega
+  have thidx : ∀ i, i < target.args.length → i < target.args.length := by omega
 
-  (stack_is_large_enough sz nargs target) ∧ ((hle : stack_is_large_enough sz nargs target) → ∀ (i : Nat), (hn : i < nargs) → stack.val[i]'(hidx hle i hn) = target.args.val[i]'(thidx i hn))
+  (stack_is_large_enough stack target) ∧ ((hle : stack_is_large_enough stack target) → ∀ (i : Nat), (hn : i < target.args.length) → stack[i]'(hidx hle i hn) = target.args[i]'(thidx i hn))
 
 @[simp]
-abbrev tail_is_compatible (sz : Nat) (stack: Stack sz) (nargs : Nat) (target : Target nargs) : Prop :=
-  ∀ (v : Var), v ∈ target.liveOut → (.Var v) ∈ stack.val.drop nargs
+abbrev tail_is_compatible (stack: List Slot) (target : Target) : Prop :=
+  ∀ (v : Var), v ∈ target.liveOut → (.Var v) ∈ stack.drop target.args.length
 
 @[simp]
-abbrev is_compatible (sz : Nat) (stack: Stack sz) (nargs : Nat) (target : Target nargs) : Prop :=
-  (stack_is_large_enough sz nargs target) ∧ (args_is_correct sz stack nargs target) ∧ (tail_is_compatible sz stack nargs target)
+abbrev is_compatible (stack: List Slot) (target : Target) : Prop :=
+  (stack_is_large_enough stack target) ∧ (args_is_correct stack target) ∧ (tail_is_compatible stack target)
 
 -- TODO: target can only be reached from stack if the variable set of target ⊆ the variable set of stack
-def shuffle (sz : Nat) (stack : Stack sz) (nargs : Nat) (target : Target nargs) : ShuffleResult :=
-  if (args_is_correct sz stack nargs target)
+def shuffle (stack : List Slot) (target : Target) : ShuffleResult :=
+  if (args_is_correct stack target)
   then
-    if (tail_is_compatible sz stack nargs target)
-    then .ResultStack sz [] stack
+    if (tail_is_compatible stack target)
+    then .ResultStack stack stack .Lit
     else .StackTooDeep
   else .StackTooDeep
 
-theorem shuffle_correct : ∀ (stack : Stack sz) (target : Target nargs), ∃ (res : ShuffleResult) (rsz : Nat) (ops : List (Π s, Op s)) (rstack : Stack rsz),
-  res = shuffle sz stack nargs target → ((.ResultStack rsz rops rstack = shuffle sz stack nargs target ∧ Stack.apply ∧ is_compatible rsz rstack nargs target) ∨ .StackTooDeep = res)
+theorem shuffle_correct : ∀ (stack : List Slot) (target : Target), ∃ (res : ShuffleResult) (rstack : List Slot) (trace : Stack.eval (.Lit stack) rstack),
+  res = shuffle stack target → ((.ResultStack stack rstack trace = shuffle stack target ∧ is_compatible rstack target) ∨ .StackTooDeep = res)
     := by
         intros stack target
-        exact ⟨.ResultStack sz [] stack, sz, [], stack , by
+        exact ⟨.ResultStack stack stack .Lit, stack, .Lit , by
           intro hres
           simp [shuffle]
           simp [shuffle] at hres
